Add type checking to spec translator.
In order to deal with things like field selection and correct treatment of references, we need type information for the translated SpecExp's. This change adds type checking to the translator and extends the test suite.

The type checking also has the added benefit that we report context errors in the spec language directly at the source instead of via the generated boogie. Right now, the tool bails out on the first type error, but the code is setup so systematic collection of errors with source level backlink can be added in subsequent PRs.

language/move-prover/bytecode-to-boogie/src/driver.rs
@@ -15,11 +15,13 @@ use libra_types::account_address::AccountAddress;
 use log::{debug, error, info};
 use std::fs;
 use std::process::Command;
+use vm::file_format::FunctionDefinitionIndex;
 
 /// Content of the default prelude.
 const DEFAULT_PRELUDE: &[u8] = include_bytes!("bytecode_instrs.bpl");
 
-/// Represents the driver for translation.
+/// Represents the driver for translation. This is the top-level object which owns
+/// all data during the steps of translation. Phases of the translation refer back to it.
 pub struct Driver<'app> {
     /// Options passed via the cli.
     options: &'app Options,
@@ -77,7 +79,7 @@ impl<'app> Driver<'app> {
     pub fn load_modules(&mut self, file_names: &[String]) {
         // TODO: make the address configurable.
         let address = AccountAddress::default();
-        for (index, file_name) in file_names.iter().enumerate() {
+        for file_name in file_names {
             info!("analyzing {}", file_name);
             // Parse module.
             let code = abort_on_error(fs::read_to_string(file_name), "cannot read mvir file");
@@ -104,7 +106,6 @@ impl<'app> Driver<'app> {
             // Store result.
             self.verified_modules.push(verified_module);
             self.module_infos.push(ModuleInfo {
-                index,
                 name,
                 function_infos: specs,
             });
@@ -115,8 +116,7 @@ impl<'app> Driver<'app> {
     /// Extract function infos from the given parsed module.
     fn extract_function_infos(&self, parsed_module: &ModuleDefinition) -> Vec<FunctionInfo> {
         let mut result = vec![];
-        for (index, (name, def)) in parsed_module.functions.iter().enumerate() {
-            let function_name = name.as_inner().as_str().to_string();
+        for (index, (_, def)) in parsed_module.functions.iter().enumerate() {
             let type_arg_names = def
                 .value
                 .signature
@@ -132,8 +132,7 @@ impl<'app> Driver<'app> {
                 .map(|(v, _)| v.value.name().as_str().to_string())
                 .collect();
             result.push(FunctionInfo {
-                index,
-                name: function_name,
+                index: FunctionDefinitionIndex(index as u16),
                 type_arg_names,
                 arg_names,
                 specification: def.value.specifications.clone(),
