language/move-prover/bytecode-to-boogie/tests/goldenfiles/test-specs.bpl
@@ -2,24 +2,48 @@
 
 // ** structs of module TestSpecs
 
+const unique TestSpecs_S: TypeName;
+const TestSpecs_S_a: FieldName;
+axiom TestSpecs_S_a == 0;
+function TestSpecs_S_type_value(): TypeValue {
+    StructType(TestSpecs_S, TypeValueArray(DefaultTypeMap[0 := AddressType()], 1))
+}
+
+procedure {:inline 1} Pack_TestSpecs_S(v0: Value) returns (v: Value)
+{
+    assume has_type(AddressType(), v0);
+    v := Struct(ValueArray(DefaultIntMap[TestSpecs_S_a := v0], 1));
+    assume has_type(TestSpecs_S_type_value(), v);
+}
+
+procedure {:inline 1} Unpack_TestSpecs_S(v: Value) returns (v0: Value)
+{
+    assert is#Struct(v);
+    v0 := smap(v)[TestSpecs_S_a];
+}
+
 const unique TestSpecs_R: TypeName;
 const TestSpecs_R_x: FieldName;
 axiom TestSpecs_R_x == 0;
+const TestSpecs_R_s: FieldName;
+axiom TestSpecs_R_s == 1;
 function TestSpecs_R_type_value(): TypeValue {
-    StructType(TestSpecs_R, TypeValueArray(DefaultTypeMap[0 := IntegerType()], 1))
+    StructType(TestSpecs_R, TypeValueArray(DefaultTypeMap[0 := IntegerType()][1 := TestSpecs_S_type_value()], 2))
 }
 
-procedure {:inline 1} Pack_TestSpecs_R(v0: Value) returns (v: Value)
+procedure {:inline 1} Pack_TestSpecs_R(v0: Value, v1: Value) returns (v: Value)
 {
     assume has_type(IntegerType(), v0);
-    v := Struct(ValueArray(DefaultIntMap[TestSpecs_R_x := v0], 1));
+    assume has_type(TestSpecs_S_type_value(), v1);
+    v := Struct(ValueArray(DefaultIntMap[TestSpecs_R_x := v0][TestSpecs_R_s := v1], 2));
     assume has_type(TestSpecs_R_type_value(), v);
 }
 
-procedure {:inline 1} Unpack_TestSpecs_R(v: Value) returns (v0: Value)
+procedure {:inline 1} Unpack_TestSpecs_R(v: Value) returns (v0: Value, v1: Value)
 {
     assert is#Struct(v);
     v0 := smap(v)[TestSpecs_R_x];
+    v1 := smap(v)[TestSpecs_R_s];
 }
 
 
@@ -49,7 +73,7 @@ procedure {:inline 1} ReadValue1(p: Path, i: int, v: Value) returns (v': Value)
     }
 }
 
-procedure {:inline 1} ReadValueMax(p: Path, i: int, v: Value) returns (v': Value)
+procedure {:inline 1} ReadValue2(p: Path, i: int, v: Value) returns (v': Value)
 {
     var e: Edge;
     if (i == size#Path(p)) {
@@ -59,6 +83,19 @@ procedure {:inline 1} ReadValueMax(p: Path, i: int, v: Value) returns (v': Value
         if (is#Struct(v)) { v' := smap(v)[f#Field(e)]; }
         if (is#Vector(v)) { v' := vmap(v)[i#Index(e)]; }
         call v' := ReadValue1(p, i+1, v');
+    }
+}
+
+procedure {:inline 1} ReadValueMax(p: Path, i: int, v: Value) returns (v': Value)
+{
+    var e: Edge;
+    if (i == size#Path(p)) {
+        v' := v;
+    } else {
+        e := p#Path(p)[i];
+        if (is#Struct(v)) { v' := smap(v)[f#Field(e)]; }
+        if (is#Vector(v)) { v' := vmap(v)[i#Index(e)]; }
+        call v' := ReadValue2(p, i+1, v');
     }
 }
 
@@ -87,7 +124,7 @@ procedure {:inline 1} UpdateValue1(p: Path, i: int, v: Value, new_v: Value) retu
     }
 }
 
-procedure {:inline 1} UpdateValueMax(p: Path, i: int, v: Value, new_v: Value) returns (v': Value)
+procedure {:inline 1} UpdateValue2(p: Path, i: int, v: Value, new_v: Value) returns (v': Value)
 {
     var e: Edge;
     if (i == size#Path(p)) {
@@ -97,6 +134,21 @@ procedure {:inline 1} UpdateValueMax(p: Path, i: int, v: Value, new_v: Value) re
         if (is#Struct(v)) { v' := smap(v)[f#Field(e)]; }
         if (is#Vector(v)) { v' := vmap(v)[i#Index(e)]; }
         call v' := UpdateValue1(p, i+1, v', new_v);
+        if (is#Struct(v)) { v' := mk_struct(smap(v)[f#Field(e) := v'], slen(v));}
+        if (is#Vector(v)) { v' := mk_vector(vmap(v)[i#Index(e) := v'], vlen(v));}
+    }
+}
+
+procedure {:inline 1} UpdateValueMax(p: Path, i: int, v: Value, new_v: Value) returns (v': Value)
+{
+    var e: Edge;
+    if (i == size#Path(p)) {
+        v' := new_v;
+    } else {
+        e := p#Path(p)[i];
+        if (is#Struct(v)) { v' := smap(v)[f#Field(e)]; }
+        if (is#Vector(v)) { v' := vmap(v)[i#Index(e)]; }
+        call v' := UpdateValue2(p, i+1, v', new_v);
         if (is#Struct(v)) { v' := mk_struct(smap(v)[f#Field(e) := v'], slen(v));}
         if (is#Vector(v)) { v' := mk_vector(vmap(v)[i#Index(e) := v'], vlen(v));}
     }
@@ -163,8 +215,8 @@ procedure TestSpecs_div_verify (arg0: Value, arg1: Value) returns (ret0: Value)
 
 procedure {:inline 1} TestSpecs_create_resource () returns ()
 requires ExistsTxnSenderAccount();
-ensures !abort_flag ==> b#Boolean(ExistsResource(gs, 1, TestSpecs_R));
-ensures !(b#Boolean(ExistsResource(gs, 1, TestSpecs_R))) ==> !abort_flag;
+ensures !abort_flag ==> b#Boolean(ExistsResource(gs, a#Address(Address(1)), TestSpecs_R));
+ensures !(b#Boolean(ExistsResource(gs, a#Address(Address(1)), TestSpecs_R))) ==> !abort_flag;
 {
     // declare local variables
 
@@ -185,4 +237,156 @@ ensures !(b#Boolean(ExistsResource(gs, 1, TestSpecs_R))) ==> !abort_flag;
 procedure TestSpecs_create_resource_verify () returns ()
 {
     call TestSpecs_create_resource();
+}
+
+procedure {:inline 1} TestSpecs_select_from_global_resource () returns ()
+requires b#Boolean(Boolean(i#Integer(SelectField(Dereference(m, GetResourceReference(gs, a#Address(Address(1)), TestSpecs_R)), TestSpecs_R_x)) > i#Integer(Integer(0))));
+requires ExistsTxnSenderAccount();
+{
+    // declare local variables
+
+    var tmp: Value;
+    var old_size: int;
+    assume !abort_flag;
+
+    // assume arguments are of correct types
+
+    old_size := m_size;
+    m_size := m_size + 0;
+
+    // bytecode translation starts here
+    return;
+
+}
+
+procedure TestSpecs_select_from_global_resource_verify () returns ()
+{
+    call TestSpecs_select_from_global_resource();
+}
+
+procedure {:inline 1} TestSpecs_select_from_resource (arg0: Value) returns (ret0: Value)
+requires b#Boolean(Boolean(i#Integer(SelectField(arg0, TestSpecs_R_x)) > i#Integer(Integer(0))));
+requires ExistsTxnSenderAccount();
+{
+    // declare local variables
+    var t0: Value; // TestSpecs_R_type_value()
+    var t1: Value; // TestSpecs_R_type_value()
+
+    var tmp: Value;
+    var old_size: int;
+    assume !abort_flag;
+
+    // assume arguments are of correct types
+    assume has_type(TestSpecs_R_type_value(), arg0);
+
+    old_size := m_size;
+    m_size := m_size + 2;
+    m := Memory(domain#Memory(m)[0+old_size := true], contents#Memory(m)[0+old_size :=  arg0]);
+
+    // bytecode translation starts here
+    call tmp := CopyOrMoveValue(contents#Memory(m)[old_size+0]);
+    m := Memory(domain#Memory(m)[1+old_size := true], contents#Memory(m)[1+old_size := tmp]);
+
+    ret0 := contents#Memory(m)[old_size+1];
+    return;
+
+}
+
+procedure TestSpecs_select_from_resource_verify (arg0: Value) returns (ret0: Value)
+{
+    call ret0 := TestSpecs_select_from_resource(arg0);
+}
+
+procedure {:inline 1} TestSpecs_select_from_resource_nested (arg0: Value) returns (ret0: Value)
+requires b#Boolean(Boolean((SelectField(SelectField(arg0, TestSpecs_R_s), TestSpecs_S_a)) == (Address(1))));
+requires ExistsTxnSenderAccount();
+{
+    // declare local variables
+    var t0: Value; // TestSpecs_R_type_value()
+    var t1: Value; // TestSpecs_R_type_value()
+
+    var tmp: Value;
+    var old_size: int;
+    assume !abort_flag;
+
+    // assume arguments are of correct types
+    assume has_type(TestSpecs_R_type_value(), arg0);
+
+    old_size := m_size;
+    m_size := m_size + 2;
+    m := Memory(domain#Memory(m)[0+old_size := true], contents#Memory(m)[0+old_size :=  arg0]);
+
+    // bytecode translation starts here
+    call tmp := CopyOrMoveValue(contents#Memory(m)[old_size+0]);
+    m := Memory(domain#Memory(m)[1+old_size := true], contents#Memory(m)[1+old_size := tmp]);
+
+    ret0 := contents#Memory(m)[old_size+1];
+    return;
+
+}
+
+procedure TestSpecs_select_from_resource_nested_verify (arg0: Value) returns (ret0: Value)
+{
+    call ret0 := TestSpecs_select_from_resource_nested(arg0);
+}
+
+procedure {:inline 1} TestSpecs_select_from_global_resource_dynamic_address (arg0: Value) returns (ret0: Value)
+requires b#Boolean(Boolean(i#Integer(SelectField(Dereference(m, GetResourceReference(gs, a#Address(SelectField(SelectField(arg0, TestSpecs_R_s), TestSpecs_S_a)), TestSpecs_R)), TestSpecs_R_x)) > i#Integer(Integer(0))));
+requires ExistsTxnSenderAccount();
+{
+    // declare local variables
+    var t0: Value; // TestSpecs_R_type_value()
+    var t1: Value; // TestSpecs_R_type_value()
+
+    var tmp: Value;
+    var old_size: int;
+    assume !abort_flag;
+
+    // assume arguments are of correct types
+    assume has_type(TestSpecs_R_type_value(), arg0);
+
+    old_size := m_size;
+    m_size := m_size + 2;
+    m := Memory(domain#Memory(m)[0+old_size := true], contents#Memory(m)[0+old_size :=  arg0]);
+
+    // bytecode translation starts here
+    call tmp := CopyOrMoveValue(contents#Memory(m)[old_size+0]);
+    m := Memory(domain#Memory(m)[1+old_size := true], contents#Memory(m)[1+old_size := tmp]);
+
+    ret0 := contents#Memory(m)[old_size+1];
+    return;
+
+}
+
+procedure TestSpecs_select_from_global_resource_dynamic_address_verify (arg0: Value) returns (ret0: Value)
+{
+    call ret0 := TestSpecs_select_from_global_resource_dynamic_address(arg0);
+}
+
+procedure {:inline 1} TestSpecs_select_from_reference (arg0: Reference) returns ()
+requires b#Boolean(Boolean((SelectField(SelectField(Dereference(m, arg0), TestSpecs_R_s), TestSpecs_S_a)) == (Address(1))));
+requires ExistsTxnSenderAccount();
+ensures b#Boolean(Boolean((SelectField(SelectField(Dereference(m, arg0), TestSpecs_R_s), TestSpecs_S_a)) == (old(SelectField(SelectField(Dereference(m, arg0), TestSpecs_R_s), TestSpecs_S_a)))));
+{
+    // declare local variables
+    var t0: Reference; // ReferenceType(TestSpecs_R_type_value())
+
+    var tmp: Value;
+    var old_size: int;
+    assume !abort_flag;
+
+    // assume arguments are of correct types
+
+    old_size := m_size;
+    m_size := m_size + 1;
+    t0 := arg0;
+
+    // bytecode translation starts here
+    return;
+
+}
+
+procedure TestSpecs_select_from_reference_verify (arg0: Reference) returns ()
+{
+    call TestSpecs_select_from_reference(arg0);
 }
